implemented the mirror shard SepExpr module type.

progs/reify_example.v
@@ -5,8 +5,217 @@ Require Import progs.list_dt.
 Require Import progs.queue.
 Local Open Scope logic.
 
+
+Module VericSepLogic <: SepTheory.SepTheory.
+
+Definition hprop := mpred.
+Definition himp := derives.
+Definition heq := fun p1 p2 => derives p1 p2 /\ derives p2 p1.
+Definition Refl_himp := derives_refl.
+Definition Trans_himp := derives_trans.
+
+Lemma Refl_heq : Reflexive heq.
+Proof. 
+intros. 
+unfold heq; split; apply derives_refl; auto.
+Qed.
+
+Lemma Sym_heq : Symmetric heq.
+Proof.
+unfold heq, Symmetric. intros.
+info intuition.
+Qed.
+
+Lemma Trans_heq : Transitive heq.
+Proof.
+unfold heq, Transitive; intros.
+intuition; eapply derives_trans; eauto.
+Qed.
+
+Local Notation "a ===> b" := (himp a b) (at level 60).
+Local Notation "a <===> b" := (heq a b) (at level 60).
+
+
+Lemma heq_defn : forall a b, (a ===> b /\ b ===> a) <-> a <===> b.
+Proof.
+intros. unfold heq, himp; intuition.
+Qed.
+
+Lemma heq_himp : forall a b, a <===> b -> a ===> b.
+Proof. intros.
+unfold heq, himp in *; intuition.
+Qed.
+
+Definition emp := emp.
+
+
+Definition inj := fun p => (prop p && emp).
+
+Definition star := sepcon.
+
+Definition ex := @exp mpred Nveric. 
+
+Lemma himp_star_comm : forall P Q, 
+    (star P Q) ===> (star Q P).
+Proof.
+intros. unfold star, himp. cancel. 
+Qed.
+
+Lemma heq_star_comm : forall P Q, 
+    (star P Q) <===> (star Q P).
+Proof.
+intros. split; unfold star; cancel.
+Qed.
+
+Lemma heq_star_assoc : forall P Q R, 
+  (star (star P Q) R) <===> (star P (star Q R)).
+Proof.
+split; unfold star; cancel.
+Qed.
+
+Lemma heq_star_emp_l : forall P, (star emp P) <===> P.
+Proof.
+split; unfold star; cancel.
+Qed.
+
+Lemma heq_star_emp_r : forall P, (star P emp) <===> P.
+Proof.
+split; unfold star; cancel.
+Qed.
+
+Lemma himp_star_frame : forall P Q R S, 
+  P ===> Q -> R ===> S -> (star P R) ===> (star Q S).
+Proof.
+intros. unfold star. unfold himp in *. apply sepcon_derives; auto.
+Qed.
+
+Ltac sep_solve :=
+  unfold star, himp, heq, emp, inj, ex in *; intuition; cancel; auto.
+
+Lemma heq_star_frame : forall P Q R S, 
+  P <===> Q -> R <===> S -> (star P R) <===> (star Q S).
+Proof.
+intros; sep_solve.
+Qed.
+
+Lemma himp_subst_p : forall P Q R S,
+  P ===> S -> (star S Q) ===> R ->
+  (star P Q) ===> R.
+Proof.
+sep_solve.
+eapply derives_trans in H0. apply H0. cancel.
+Qed.
+
+Lemma himp_subst_c : forall P Q R S,
+  S ===> Q -> P ===> (star S R) ->
+  P ===> (star Q R).
+Proof.
+sep_solve.
+eapply derives_trans; eauto; cancel.
+Qed.
+
+Lemma heq_subst : forall P Q R S,
+  P <===> S -> (star S Q) <===> R ->
+  (star P Q) <===> R.
+Proof.
+sep_solve.
+eapply derives_trans in H; eauto; cancel.
+eapply derives_trans; eauto; cancel.
+Qed.
+
+Lemma himp_star_cancel : forall P Q R,
+  Q ===> R -> (star P Q) ===> (star P R).
+Proof.
+sep_solve.
+Qed.
+
+Lemma heq_star_cancel : forall P Q R, 
+  Q <===> R -> (star P Q) <===> (star P R).
+Proof.
+sep_solve.
+Qed.
+
+
+(** pure lemmas **)
+Lemma himp_star_pure_p : forall P Q F,
+  (star (inj F) P) ===> Q -> (F -> P ===> Q).
+Proof.
+sep_solve.
+eapply derives_trans in H; eauto; entailer!.
+Qed.
+
+Lemma himp_star_pure_c : forall P Q (F : Prop),
+  (F -> P ===> Q) -> (star (inj F) P) ===> Q.
+Proof.
+intros.
+sep_solve. entailer!.
+Qed.
+
+  Lemma himp_star_pure_cc : forall P Q (p : Prop),
+    p ->
+    P ===> Q ->
+    P ===> (star (inj p) Q).
+Proof.
+sep_solve. entailer!.
+Qed.
+
+  (** ex lemmas **)
+  Lemma himp_ex_p : forall T (P : T -> _) Q, 
+            (forall v, (P v) ===> Q) -> (ex T P) ===> Q.
+  Proof. sep_solve. apply exp_left. auto.
+Qed.
+
+  Lemma himp_ex_c : forall T (P : T -> _) Q, 
+    (exists v, Q ===> (P v)) -> Q ===> (ex T P).
+  Proof. 
+ sep_solve. destruct H. eapply exp_right.  apply H.
+Qed.
+
+  Lemma heq_ex : forall T (P Q : T -> _), 
+    (forall v, P v <===> Q v) ->
+    ex T P <===> ex T Q.
+Proof. 
+sep_solve; apply exp_left;  intros;
+specialize (H x); destruct H; apply (exp_right x);
+auto.
+Qed.
+
+  Lemma himp_ex : forall T (P Q : T -> _), 
+    (forall v, P v ===> Q v) ->
+    ex T P ===> ex T Q.
+Proof.
+sep_solve. apply exp_left. intros.
+specialize (H x). apply (exp_right x). auto.
+Qed.
+
+  Lemma heq_ex_star : forall T (P : T -> _) Q,
+    (star (ex T P) Q) <===> (ex T (fun x => star (P x) Q)).
+Proof.
+sep_solve. entailer!.
+entailer!. apply (exp_right x). auto.
+Qed.
+
+  Lemma himp_ex_star : forall T (P : T -> _) Q,
+    (star (ex T P) Q) ===> (ex T (fun x => star (P x) Q)).
+Proof.
+sep_solve. entailer!.
+Qed.
+
+End VericSepLogic.
+
+Check derives_extract_prop.
+Print SepExpr.SepExpr.
+Module Sep := SepExpr.Make VericSepLogic.
+
+
+(*Definition if_then_else_isnil (b : forall (s: list val), {s=nil}+{s<>nil})
+(m1 m2 : mpred) := if b then m1 else m2.
+*)
 Lemma isnil: forall {T: Type} (s: list T), {s=nil}+{s<>nil}.
 Proof. intros. destruct s; [left|right]; auto. intro Hx; inv Hx. Qed.
+
+Check (isnil nil).
+
 
 Instance QS: listspec t_struct_elem _next. 
 Proof. eapply mk_listspec; reflexivity. Defined.
@@ -257,6 +466,9 @@ Definition environ2prop_type_var := Expr.tvType 5.
 
 Definition delta_const := @Expr.Const our_types tycontext_type_var Delta.
 
+
+(*above preconstructed, below constructed by entailer *)
+
 Definition c_option_expr_const := @Expr.Const our_types c_option_expr_type_var 
 (@Some expr
             (Ebinop Oeq (Etempvar _h (tptr t_struct_elem))
@@ -272,22 +484,18 @@ Expr.Sig our_types (cons tycontext_type_var (cons c_option_expr_type_var (cons c
 Definition tc_expropt_signature : Expr.signature our_types :=
 Expr.Sig our_types (cons tycontext_type_var (cons c_option_expr_type_var (cons c_type_type_var (cons environ_type_var nil)))) prop_type_var tc_expropt.
 
-Definition functions := cons ret_type_signature
+
+Definition environ_signature (rho: environ) : Expr.signature our_types :=
+Expr.Sig our_types (nil) (environ_type_var) (rho).
+
+Definition functions (rho:environ) := cons ret_type_signature
                        (cons tc_expropt_signature
-                       (cons tc_expropt_signature_lifted nil)).
+                       (cons tc_expropt_signature_lifted 
+                       (cons (environ_signature rho) nil))).
 
 Definition ret_type_delta : Expr.expr our_types.
 eapply Expr.Func. apply 0%nat. apply (cons delta_const nil).
 Defined.
-
-Compute (Expr.exprD (functions) nil nil  ret_type_delta c_type_type_var).
-
-Check tc_expropt.
-
-Print Expr.tvar.
-
-
-Check tc_expropt_signature.
 
 Definition tc_expropt_application_lifted : Expr.expr our_types.
 eapply Expr.Func.
@@ -299,21 +507,8 @@ Definition tc_expropt_application_unlifted : Expr.expr our_types.
 eapply Expr.Func.
 apply 1%nat.
 apply (cons delta_const (cons c_option_expr_const (cons ret_type_delta 
-                                                       (cons (Expr.Var 0%nat) nil)))).
+                                                       (cons (Expr.Func 3%nat nil) nil)))).
 Defined.
-
-Definition vars : Expr.env our_types.
-unfold Expr.env.
-apply cons; [ | apply nil].
-unfold Expr.tvarD.
-Set Printing All.
-SearchAbout sigT.
-exists environ_type_var. simpl.
-apply empty_environ.
-apply semax_lemmas.empty_genv.
-Qed.
-
-Print vars. Check projT1.
 
 Definition reflected_tc_expropt :=
 (tc_expropt Delta
@@ -330,36 +525,256 @@ forall rho,
                (Ecast (Econst_int (Int.repr 0) tint) (tptr tvoid)) tint))
          (ret_type Delta) rho).
 
+Lemma tc_expropt_true : 
+forall rho,
+tc_environ Delta rho ->
+(tc_expropt Delta
+         (@Some expr
+            (Ebinop Oeq (Etempvar _h (tptr t_struct_elem))
+               (Ecast (Econst_int (Int.repr 0) tint) (tptr tvoid)) tint))
+         (ret_type Delta) rho).
+Proof.
+intros. simpl.
+unfold tc_expr. simpl. super_unfold_lift.
+pose (funcs := functions rho).
+assert  (Some (tc_expropt Delta
+     (Some
+        (Ebinop Oeq (Etempvar _h (tptr t_struct_elem))
+           (Ecast (Econst_int (Int.repr 0) tint) (tptr tvoid)) tint))
+     (ret_type Delta) rho) = 
+Expr.exprD funcs nil nil tc_expropt_application_unlifted prop_type_var).
+auto.
 
-Lemma tc_expropt_reify_reflect_unlifted : (Expr.exprD functions nil vars tc_expropt_application_unlifted 
-prop_type_var) = Some reflected_tc_expropt_unlifted.
-simpl. unfold Expr.lookupAs. simpl.
-Check vars.
-Check projT1.
-Locate value
-Print vars.
-unfold tc_expropt_application_unlifted.
-unfold Expr.exprD.
-simpl (nth_error functions 1).
-unfold value.
-unfold Expr.Range.
-unfold tc_expropt_signature.
-intros. simpl. auto.
+Definition prove_goal (exp : Expr.expr our_types) := false.
+
+Definition work_on_goal (exp : Expr.expr our_types) := exp.
+
+Lemma work_on_goal_sound :
+forall exp exp2 f p p2,
+work_on_goal exp = exp2 ->
+Expr.exprD f nil nil exp prop_type_var = Some p ->
+(Expr.exprD f nil nil exp2 prop_type_var = Some p2 /\ (p2 -> p)).
+Proof. admit.
 Qed.
 
-Lemma tc_expropt_reify_reflect : (Expr.exprD functions nil nil tc_expropt_application_lifted 
-environ2prop_type_var) = Some reflected_tc_expropt.
-intros. simpl. auto.
+Lemma prove_goal_sound : 
+forall exp f p,
+prove_goal exp = true ->
+Expr.exprD f nil nil exp prop_type_var = Some p ->
+p.
+Proof.
+intros. inv H.
+Qed.
+
+ 
+assert ((prove_goal tc_expropt_application_unlifted = true)) by admit.
+eapply prove_goal_sound.
+apply H1.
+symmetry in H0. apply H0.
 Qed.
 
 
+Lemma goal_1 :
+name _Q ->
+name _h ->
+forall (q : val) (contents : list val) (hd tl : val),
+let Delta :=
+  @abbreviate tycontext
+    (initialized _h
+       (@PTree.Node (type * bool)
+          (@PTree.Node (type * bool) (@PTree.Leaf (type * bool))
+             (@None (type * bool))
+             (@PTree.Node (type * bool) (@PTree.Leaf (type * bool))
+                (@None (type * bool))
+                (@PTree.Node (type * bool)
+                   (@PTree.Node (type * bool) (@PTree.Leaf (type * bool))
+                      (@Some (type * bool) (tptr t_struct_elem, false))
+                      (@PTree.Leaf (type * bool))) (@None (type * bool))
+                   (@PTree.Leaf (type * bool))))) (@None (type * bool))
+          (@PTree.Node (type * bool) (@PTree.Leaf (type * bool))
+             (@None (type * bool))
+             (@PTree.Node (type * bool)
+                (@PTree.Node (type * bool)
+                   (@PTree.Node (type * bool) (@PTree.Leaf (type * bool))
+                      (@Some (type * bool) (tptr t_struct_fifo, true))
+                      (@PTree.Leaf (type * bool))) (@None (type * bool))
+                   (@PTree.Leaf (type * bool))) (@None (type * bool))
+                (@PTree.Leaf (type * bool)))), PTree.empty type, tint,
+       @PTree.Node global_spec
+         (@PTree.Node global_spec
+            (@PTree.Node global_spec
+               (@PTree.Node global_spec (@PTree.Leaf global_spec)
+                  (@Some global_spec
+                     (Global_func
+                        (WITH _ : unit PRE  [(1%positive, tptr tvoid),
+                         (2%positive, tptr tvoid), (3%positive, tuint),
+                         (4%positive, tuint)](fun _ : environ => !!False)
+                         POST  [tvoid](fun _ : environ => !!False))))
+                  (@PTree.Node global_spec (@PTree.Leaf global_spec)
+                     (@Some global_spec
+                        (Global_func
+                           (WITH  p0 : val * list val, p : val PRE 
+                            [(_Q, tptr t_struct_fifo),
+                            (_p, tptr t_struct_elem)]
+                            (let (q0, contents0) := p0 in
+                             PROP  ()
+                             LOCAL  (`(@eq val q0) (eval_id _Q);
+                             `(@eq val p) (eval_id _p))
+                             SEP  (`(fifo contents0 q0); `(link_ p))) POST 
+                            [tvoid]
+                            (let (q0, contents0) := p0 in
+                             `(fifo (contents0 ++ p :: @nil val) q0)))))
+                     (@PTree.Leaf global_spec))) (@None global_spec)
+               (@PTree.Node global_spec
+                  (@PTree.Node global_spec (@PTree.Leaf global_spec)
+                     (@Some global_spec
+                        (Global_func
+                           (WITH _ : unit PRE  []
+                            (fun _ : environ => @emp mpred Nveric Sveric)
+                            POST  [tptr t_struct_fifo]
+                            `(fifo (@nil val)) retval)))
+                     (@PTree.Leaf global_spec)) (@None global_spec)
+                  (@PTree.Node global_spec (@PTree.Leaf global_spec)
+                     (@Some global_spec
+                        (Global_func
+                           (WITH  a : int, b : int PRE  [(_a, tint),
+                            (_b, tint)]
+                            PROP  ()
+                            LOCAL  (`(@eq val (Vint a)) (eval_id _a);
+                            `(@eq val (Vint b)) (eval_id _b))  SEP() POST 
+                            [tptr t_struct_elem]`(elemrep (a, b)) retval)))
+                     (@PTree.Leaf global_spec)))) (@None global_spec)
+            (@PTree.Node global_spec
+               (@PTree.Node global_spec (@PTree.Leaf global_spec)
+                  (@Some global_spec
+                     (Global_func
+                        (WITH n : int PRE  [(1%positive, tint)]
+                         PROP  (4 <= Int.signed n)
+                         LOCAL  (`(@eq val (Vint n)) (eval_id 1%positive))
+                         SEP() POST  [tptr tvoid]`(memory_block Tsh n) retval)))
+                  (@PTree.Leaf global_spec)) (@None global_spec)
+               (@PTree.Leaf global_spec))) (@None global_spec)
+         (@PTree.Node global_spec
+            (@PTree.Node global_spec
+               (@PTree.Node global_spec (@PTree.Leaf global_spec)
+                  (@Some global_spec
+                     (Global_func
+                        (WITH _ : unit PRE  [(1%positive, tptr tschar),
+                         (2%positive, tint)](fun _ : environ => !!False)
+                         POST  [tint](fun _ : environ => !!False))))
+                  (@PTree.Node global_spec (@PTree.Leaf global_spec)
+                     (@Some global_spec
+                        (Global_func
+                           (WITH  q0 : val, contents0 : list val PRE 
+                            [(_Q, tptr t_struct_fifo)]
+                            PROP  ()
+                            LOCAL  (`(@eq val q0) (eval_id _Q))
+                            SEP  (`(fifo contents0 q0)) POST  [tint]
+                            (fun x0 : environ =>
+                             local
+                               (`(@eq val
+                                    (if @isnil val contents0
+                                     then Vtrue
+                                     else Vfalse)) retval) x0 &&
+                             `(fifo contents0 q0) x0))))
+                     (@PTree.Leaf global_spec))) (@None global_spec)
+               (@PTree.Leaf global_spec)) (@None global_spec)
+            (@PTree.Node global_spec
+               (@PTree.Node global_spec (@PTree.Leaf global_spec)
+                  (@Some global_spec
+                     (Global_func
+                        (WITH _ : unit PRE  [(1%positive, tptr tvoid),
+                         (2%positive, tint)]
+                         PROP  ()
+                         LOCAL ()
+                         SEP 
+                         (`(memory_block Tsh)
+                            (`force_int (eval_id 2%positive))
+                            (eval_id 1%positive)) POST  [tvoid]
+                         (fun _ : environ => @emp mpred Nveric Sveric))))
+                  (@PTree.Node global_spec (@PTree.Leaf global_spec)
+                     (@Some global_spec
+                        (Global_func
+                           (WITH  p0 : val * list val, p : val PRE 
+                            [(_Q, tptr t_struct_fifo)]
+                            (let (q0, contents0) := p0 in
+                             PROP  ()
+                             LOCAL  (`(@eq val q0) (eval_id _Q))
+                             SEP  (`(fifo (p :: contents0) q0))) POST 
+                            [tptr t_struct_elem]
+                            (let (q0, contents0) := p0 in
+                             fun rho : environ =>
+                             local (`(@eq val p) retval) rho &&
+                             `(fifo contents0 q0) rho * `link_ retval rho))))
+                     (@PTree.Leaf global_spec)))
+               (@Some global_spec
+                  (Global_func
+                     (WITH _ : unit PRE  [(1%positive, tdouble)]
+                      (fun _ : environ => !!False) POST  [tdouble]
+                      (fun _ : environ => !!False))))
+               (@PTree.Node global_spec (@PTree.Leaf global_spec)
+                  (@None global_spec)
+                  (@PTree.Node global_spec (@PTree.Leaf global_spec)
+                     (@Some global_spec
+                        (Global_func
+                           (WITH u : unit PRE  []main_pre prog u POST  [tint]
+                            main_post prog u))) (@PTree.Leaf global_spec))))))) in
+PROP  ()
+LOCAL  (tc_environ Delta; `(@eq val hd) (eval_id _h);
+`(@eq val q) (eval_id _Q))
+SEP  (`(field_mapsto Tsh t_struct_fifo _head q hd);
+`(field_mapsto Tsh t_struct_fifo _tail q tl);
+`(if @isnil val contents
+  then !!(hd = nullval) && @emp mpred Nveric Sveric
+  else
+   EX  prefix : list val,
+   !!(contents = prefix ++ tl :: @nil val) &&
+   (@links t_struct_elem _next QS Tsh prefix hd tl * link tl nullval)))
+|-- local
+      (tc_expropt Delta
+         (@Some expr
+            (Ebinop Oeq (Etempvar _h (tptr t_struct_elem))
+               (Ecast (Econst_int (Int.repr 0) tint) (tptr tvoid)) tint))
+         (ret_type Delta)) &&
+    `(function_body_ret_assert tint
+        (local
+           (`(@eq val (if @isnil val contents then Vtrue else Vfalse)) retval) &&
+         `(fifo contents q)) EK_return)
+      (cast_expropt
+         (@Some expr
+            (Ebinop Oeq (Etempvar _h (tptr t_struct_elem))
+               (Ecast (Econst_int (Int.repr 0) tint) (tptr tvoid)) tint))
+         (ret_type Delta)) (@id environ)
+. Proof. intros Q h.
+ ungather_entail.
+unfold fifo. 
+go_lower.
 
+Check Expr.Func.
+
+Definition saturate (exps: ((list Expr.expr) * Expr.expr)) : bool :=
+let exps := (assumptions, goal) in
+match with 
+ ...
+| Exps.Func n exps =>
+     if eqb_nat n 5 then 
+             sat
+     else 
+         .... 
+
+
+entailer.
+apply exp_right with (h,tl).
+entailer.
+if_tac; entailer; elim_hyps; simpl; auto.
+destruct prefix; entailer1.
+Qed.
 
 
 
 
 (* 
 *** Local Variables: ***
-*** coq-load-path: (("../coq-ext-lib/theories" "ExtLib") ("." "MirrorShard") "../../../work/vst/" "../../../work/floyd" "../../../work/progs") ***
+*** coq-load-path: (("../../../GitHub/coq-ext-lib/theories" "ExtLib") ("../../../GitHub/mirror-shard/src" "MirrorShard") ("../veric/" "veric") ("../floyd" "floyd") ("../progs" "progs") ("../compcert" "compcert") ("../msl" "msl") ("../sepcomp" "sepcomp")) ***
 *** End: ***
 *)
